Handle the new Or gate in xaig_to_cnf
Or is the dual of And throughout, so it slots in alongside it:

  gty_pos m (Or ts)  one clause  m ⇒ l1 ∨ ... ∨ lk
  gty_neg m (Or ts)  k clauses   li ⇒ m

which mirrors And's k clauses one way and single clause the other. Or is
monotone in all of its inputs, so like And it passes its own polarity on
to each of them, and renaming treats it exactly as it treats And (the
reversal the accumulator introduces is as harmless for a disjunction as
it is for a conjunction).

xrename_lits_thm now also states the EXISTS form of its conclusion,
which is what the Or case of xrename_gty_thm needs where the And case
uses the EVERY form.

Co-Authored-By: Claude <noreply@anthropic.com>

examples/hwmcc_checker/xaig_to_cnfScript.sml
@@ -17,6 +17,12 @@ Proof
   Induct_on ‘xs’ \\ fs []
 QED
 
+Theorem EXISTS_EQ_EXISTS[local]:
+  EVERY (λx. P x = Q x) xs ⇒ (EXISTS P xs = EXISTS Q xs)
+Proof
+  Induct_on ‘xs’ \\ fs []
+QED
+
 Theorem FUNION_SUBMAP_lemma[local]:
   im_1 SUBMAP im_2 ⇒
   (im_1 ⊌ im_2 = im_2) ∧
@@ -43,7 +49,8 @@ QED
 Definition gty_lits_def[simp]:
   gty_lits (And ts) = ts ∧
   gty_lits (Xor t1 t2) = [t1; t2] ∧
-  gty_lits (Ite t1 t2 t3) = [t1; t2; t3]
+  gty_lits (Ite t1 t2 t3) = [t1; t2; t3] ∧
+  gty_lits (Or ts) = ts
 End
 
 Theorem xeval_gty_cong:
@@ -52,7 +59,8 @@ Theorem xeval_gty_cong:
     (xeval_gty ss xs gt ⇔ xeval_gty ss' ys gt)
 Proof
   Cases \\ simp [xeval_lit_def] \\ strip_tac \\ gvs []
-  \\ irule EVERY_EQ_EVERY \\ fs []
+  >- (irule EVERY_EQ_EVERY \\ fs [])
+  \\ irule EXISTS_EQ_EXISTS \\ fs []
 QED
 
 Theorem xeval_gate_nil[simp]:
@@ -182,8 +190,9 @@ Definition xrename_lit_def:
 End
 
 (* Note that this accumulates the renamed literals in reverse order. That
-   is harmless: the only gates built from a list of literals are And gates,
-   i.e. conjunctions.  Accumulating makes this function tail recursive. *)
+   is harmless: the only gates built from a list of literals are And and Or
+   gates, and neither cares about the order of its inputs.  Accumulating
+   makes this function tail recursive. *)
 
 Definition xrename_lits_def:
   xrename_lits ([]:('a,'i,'l) aig$lit list) next im lm nm acc =
@@ -217,7 +226,10 @@ Definition xrename_gty_def:
     (let (u1,next,im,lm) = xrename_lit t1 next im lm nm in
      let (u2,next,im,lm) = xrename_lit t2 next im lm nm in
      let (u3,next,im,lm) = xrename_lit t3 next im lm nm in
-       (Ite u1 u2 u3,next,im,lm))
+       (Ite u1 u2 u3,next,im,lm)) ∧
+  xrename_gty (Or ts) next im lm nm =
+    (let (ts1,next,im,lm) = xrename_lits ts next im lm nm [] in
+       (Or ts1,next,im,lm))
 End
 
 Definition xaig_rename_def:
@@ -461,7 +473,10 @@ Theorem xrename_lits_thm:
     (∀m b. MEM (Gate m,b) ts_1 ⇒ m ∈ FRANGE nm) ∧
     wrt_ext im_2 lm_2
       (λi l. EVERY (xeval_lit (is,ls) xaig) ts =
-             EVERY (xeval_lit (aig_read is i, aig_read ls l) res) ts_1)
+             EVERY (xeval_lit (aig_read is i, aig_read ls l) res) ts_1) ∧
+    wrt_ext im_2 lm_2
+      (λi l. EXISTS (xeval_lit (is,ls) xaig) ts =
+             EXISTS (xeval_lit (aig_read is i, aig_read ls l) res) ts_1)
 Proof
   Induct >- (fs [xrename_lits_def] \\ rw [] \\ simp [wrt_ext_def])
   \\ rpt gen_tac \\ simp [xrename_lits_def]
@@ -483,7 +498,7 @@ Proof
   >- (rw [] \\ imp_res_tac SUBMAP_FRANGE \\ res_tac \\ fs [SUBSET_DEF])
   >- (rw [] \\ res_tac)
   \\ fs [wrt_ext_def] \\ rw [] \\ res_tac
-  \\ simp [AC CONJ_COMM CONJ_ASSOC]
+  \\ simp [AC CONJ_COMM CONJ_ASSOC, AC DISJ_COMM DISJ_ASSOC]
 QED
 
 Theorem xrename_gty_thm:
@@ -528,34 +543,37 @@ Proof
     >- (rw [] \\ res_tac)
     \\ fs [wrt_ext_def] \\ rw [] \\ res_tac \\ simp [])
   (* if-then-else gates *)
-  \\ qpat_x_assum ‘xrename_lit p _ _ _ _ = _’ assume_tac
-  \\ drule_all xrename_lit_thm \\ strip_tac
-  \\ qpat_x_assum ‘xrename_lit p0 _ _ _ _ = _’ assume_tac
-  \\ drule_all xrename_lit_thm \\ strip_tac
-  \\ qpat_x_assum ‘xrename_lit p1 _ _ _ _ = _’ assume_tac
-  \\ drule_all xrename_lit_thm \\ strip_tac
-  \\ ‘im_1 SUBMAP im'' ∧ lm_1 SUBMAP lm'' ∧ im SUBMAP im'' ∧ lm SUBMAP lm''’ by
-       metis_tac [SUBMAP_TRANS]
-  \\ simp []
-  \\ ‘wrt_ext im'' lm''
-        (λi l. xeval_lit (is,ls) xaig p ⇔
-               xeval_lit (aig_read is i,aig_read ls l) res u1)’ by
-       (irule wrt_ext_mono
-        \\ qpat_x_assum ‘wrt_ext im lm _’ $ irule_at Any \\ simp [])
-  \\ ‘wrt_ext im'' lm''
-        (λi l. xeval_lit (is,ls) xaig p0 ⇔
-               xeval_lit (aig_read is i,aig_read ls l) res u2)’ by
-       (irule wrt_ext_mono
-        \\ qpat_x_assum ‘wrt_ext im' lm' _’ $ irule_at Any \\ simp [])
-  \\ rpt conj_tac
-  >- (rw [] \\ res_tac \\ fs [SUBMAP_DEF])
-  >- (rw [] \\ res_tac \\ fs [SUBMAP_DEF])
-  >- (rw [] \\ imp_res_tac SUBMAP_FRANGE \\ res_tac \\ fs [SUBSET_DEF])
-  >- (rw [] \\ imp_res_tac SUBMAP_FRANGE \\ res_tac \\ fs [SUBSET_DEF])
-  >- (rw [] \\ res_tac)
-  \\ fs [wrt_ext_def] \\ rw [] \\ res_tac \\ simp []
+  >-
+   (qpat_x_assum ‘xrename_lit p _ _ _ _ = _’ assume_tac
+    \\ drule_all xrename_lit_thm \\ strip_tac
+    \\ qpat_x_assum ‘xrename_lit p0 _ _ _ _ = _’ assume_tac
+    \\ drule_all xrename_lit_thm \\ strip_tac
+    \\ qpat_x_assum ‘xrename_lit p1 _ _ _ _ = _’ assume_tac
+    \\ drule_all xrename_lit_thm \\ strip_tac
+    \\ ‘im_1 SUBMAP im'' ∧ lm_1 SUBMAP lm'' ∧
+        im SUBMAP im'' ∧ lm SUBMAP lm''’ by metis_tac [SUBMAP_TRANS]
+    \\ simp []
+    \\ ‘wrt_ext im'' lm''
+          (λi l. xeval_lit (is,ls) xaig p ⇔
+                 xeval_lit (aig_read is i,aig_read ls l) res u1)’ by
+         (irule wrt_ext_mono
+          \\ qpat_x_assum ‘wrt_ext im lm _’ $ irule_at Any \\ simp [])
+    \\ ‘wrt_ext im'' lm''
+          (λi l. xeval_lit (is,ls) xaig p0 ⇔
+                 xeval_lit (aig_read is i,aig_read ls l) res u2)’ by
+         (irule wrt_ext_mono
+          \\ qpat_x_assum ‘wrt_ext im' lm' _’ $ irule_at Any \\ simp [])
+    \\ rpt conj_tac
+    >- (rw [] \\ res_tac \\ fs [SUBMAP_DEF])
+    >- (rw [] \\ res_tac \\ fs [SUBMAP_DEF])
+    >- (rw [] \\ imp_res_tac SUBMAP_FRANGE \\ res_tac \\ fs [SUBSET_DEF])
+    >- (rw [] \\ imp_res_tac SUBMAP_FRANGE \\ res_tac \\ fs [SUBSET_DEF])
+    >- (rw [] \\ res_tac)
+    \\ fs [wrt_ext_def] \\ rw [] \\ res_tac \\ simp [])
+  (* multi-input or gates *)
+  \\ drule_all xrename_lits_thm \\ strip_tac \\ fs [SF ETA_ss]
+  \\ rw [] \\ res_tac
 QED
-
 Theorem xaig_rename_thm:
   ∀(xaig:('a,'i,'l) xaig) res next im lm nm.
     xaig_rename xaig = (res,next,im,lm,nm) ⇒
@@ -698,6 +716,14 @@ Definition eq_every_neg_def:
   eq_every_neg x xs = [x::MAP negate xs]
 End
 
+Definition or_every_pos_def:
+  or_every_pos x xs = [negate x :: xs]
+End
+
+Definition or_every_neg_def:
+  or_every_neg x xs = MAP (λy. [negate y; x]) xs
+End
+
 Definition xor_pos_def:
   xor_pos y a b = [[negate y; a; b]; [negate y; negate a; negate b]]
 End
@@ -718,14 +744,16 @@ Definition gty_pos_def:
   gty_pos m (And ts) = eq_every_pos (Pos m) (MAP var_to_lit ts) ∧
   gty_pos m (Xor t1 t2) = xor_pos (Pos m) (var_to_lit t1) (var_to_lit t2) ∧
   gty_pos m (Ite t1 t2 t3) =
-    ite_pos (Pos m) (var_to_lit t1) (var_to_lit t2) (var_to_lit t3)
+    ite_pos (Pos m) (var_to_lit t1) (var_to_lit t2) (var_to_lit t3) ∧
+  gty_pos m (Or ts) = or_every_pos (Pos m) (MAP var_to_lit ts)
 End
 
 Definition gty_neg_def:
   gty_neg m (And ts) = eq_every_neg (Pos m) (MAP var_to_lit ts) ∧
   gty_neg m (Xor t1 t2) = xor_neg (Pos m) (var_to_lit t1) (var_to_lit t2) ∧
   gty_neg m (Ite t1 t2 t3) =
-    ite_neg (Pos m) (var_to_lit t1) (var_to_lit t2) (var_to_lit t3)
+    ite_neg (Pos m) (var_to_lit t1) (var_to_lit t2) (var_to_lit t3) ∧
+  gty_neg m (Or ts) = or_every_neg (Pos m) (MAP var_to_lit ts)
 End
 
 (* both halves together are the usual Tseitin clauses for the gate *)
@@ -785,6 +813,17 @@ Proof
   \\ Cases_on ‘satisfies_lit w b’ \\ fs []
 QED
 
+Theorem or_to_cnf_thm[local]:
+  satisfies_cnf w (set (or_every_pos y xs) ∪ set (or_every_neg y xs)) ⇔
+  (satisfies_lit w y ⇔ EXISTS (satisfies_lit w) xs)
+Proof
+  simp [satisfies_cnf_def, satisfies_fml_gen_def, or_every_pos_def,
+        or_every_neg_def, satisfies_clause_def, satisfies_lit_negate,
+        MEM_MAP, EXISTS_MEM, SF DNF_ss]
+  \\ Cases_on ‘satisfies_lit w y’ \\ simp []
+  \\ metis_tac []
+QED
+
 Theorem set_eq_every[local]:
   set (eq_every_pos x xs) ∪ set (eq_every_neg x xs) =
   set (eq_every_to_cnf x xs)
@@ -805,7 +844,9 @@ Proof
         xeval_lit_def]
     \\ AP_TERM_TAC \\ irule EVERY_EQ_EVERY \\ fs [])
   >- fs [xor_to_cnf_thm, satisfies_lit_def, xeval_lit_def]
-  \\ fs [ite_to_cnf_thm, satisfies_lit_def, xeval_lit_def]
+  >- fs [ite_to_cnf_thm, satisfies_lit_def, xeval_lit_def]
+  \\ fs [or_to_cnf_thm, satisfies_lit_def, EXISTS_MAP, xeval_lit_def]
+  \\ AP_TERM_TAC \\ irule EXISTS_EQ_EXISTS \\ fs []
 QED
 
 (* Polarities.  A polarity (p,n) records whether a gate name is used
@@ -846,7 +887,8 @@ End
 Definition gty_pols_def:
   gty_pols pl (And ts) = MAP (λt. (pl,t)) ts ∧
   gty_pols pl (Xor t1 t2) = [((T,T),t1); ((T,T),t2)] ∧
-  gty_pols pl (Ite t1 t2 t3) = [((T,T),t1); (pl,t2); (pl,t3)]
+  gty_pols pl (Ite t1 t2 t3) = [((T,T),t1); (pl,t2); (pl,t3)] ∧
+  gty_pols pl (Or ts) = MAP (λt. (pl,t)) ts
 End
 
 Definition add_lits_pol_def:
@@ -993,8 +1035,11 @@ Proof
   >-
    (fs [EVERY_MEM] \\ rw [] \\ res_tac
     \\ irule lit_pol_ok_mono \\ first_assum $ irule_at Any \\ simp [])
-  \\ conj_tac \\ irule lit_pol_ok_mono
-  \\ first_assum $ irule_at Any \\ simp []
+  >-
+   (conj_tac \\ irule lit_pol_ok_mono
+    \\ first_assum $ irule_at Any \\ simp [])
+  \\ fs [EVERY_MEM] \\ rw [] \\ res_tac
+  \\ irule lit_pol_ok_mono \\ first_assum $ irule_at Any \\ simp []
 QED
 
 Theorem satisfies_lit_Pos[local,simp]:
@@ -1012,9 +1057,12 @@ Proof
   Cases
   \\ simp [gty_pos_def, gty_pols_def, satisfies_cnf_set, satisfies_clause_def,
            satisfies_lit_negate, eq_every_pos_def, xor_pos_def, ite_pos_def,
-           EVERY_MAP, SF DNF_ss, xeval_lit_def, lit_pol_ok_def]
+           or_every_pos_def, EVERY_MAP, EXISTS_MAP, MEM_MAP, SF DNF_ss,
+           xeval_lit_def, lit_pol_ok_def]
   >- (rw [EVERY_MEM] \\ res_tac \\ gvs [])
-  \\ rw [] \\ metis_tac []
+  >- (rw [] \\ metis_tac [])
+  >- (rw [] \\ metis_tac [])
+  \\ rw [EXISTS_MEM, EVERY_MEM] \\ res_tac \\ metis_tac []
 QED
 
 Theorem gty_neg_thm[local]:
@@ -1026,9 +1074,12 @@ Proof
   Cases
   \\ simp [gty_neg_def, gty_pols_def, satisfies_cnf_set, satisfies_clause_def,
            satisfies_lit_negate, eq_every_neg_def, xor_neg_def, ite_neg_def,
-           EVERY_MAP, MEM_MAP, SF DNF_ss, xeval_lit_def, lit_pol_ok_def]
+           or_every_neg_def, EVERY_MAP, EXISTS_MAP, MEM_MAP, SF DNF_ss,
+           xeval_lit_def, lit_pol_ok_def]
   >- (rw [EVERY_MEM] \\ res_tac \\ gvs [])
-  \\ rw [] \\ metis_tac []
+  >- (rw [] \\ metis_tac [])
+  >- (rw [] \\ metis_tac [])
+  \\ rw [EXISTS_MEM, EVERY_MEM] \\ res_tac \\ metis_tac []
 QED
 
 Theorem pol_le_FST_SND[local]:
@@ -1285,7 +1336,7 @@ Proof
   Cases_on ‘gt’
   \\ fs [gty_pos_def, gty_neg_def, lits_within_def, eq_every_pos_def,
          eq_every_neg_def, xor_pos_def, xor_neg_def, ite_pos_def, ite_neg_def,
-         EVERY_MAP]
+         or_every_pos_def, or_every_neg_def, EVERY_MAP]
 QED
 
 Theorem lits_within_xgty_to_cnf[local]:
